Remove well-formed conditions

KripkeMetatheory.v
@@ -3,55 +3,27 @@ Require Import Classical.
 
 Require Import Flowers.Syntax Flowers.KripkeSemantics Flowers.Utils.
 
-Context (Σ : sig).
-
 (** * Soundness *)
 
 Section Soundness.
 
 Context A (K : KModel A).
 
-Lemma local_soundness (Φ Ψ : wfbouquet) :
+Lemma local_soundness (Φ Ψ : bouquet) :
   Φ ⇀ Ψ -> Φ ⫤⊨ Ψ.
 Admitted.
 
-Lemma grounding : ∀ (X : wfctx) (Φ Ψ : wfbouquet),
-  Φ ⫤⊨ Ψ -> btot (X ⋖ Φ ⇂ wf_fill X Φ) ⫤⊨ btot (X ⋖ Ψ ⇂ wf_fill X Ψ).
+Lemma grounding : ∀ (X : ctx) (Φ Ψ : bouquet),
+  Φ ⫤⊨ Ψ -> X ⋖ Φ ⫤⊨ X ⋖ Ψ.
 Admitted.
 
-Lemma pgrounding : ∀ (P : wfpctx) (Φ Ψ : wfbouquet),
-  Φ ⊨ Ψ -> btot (P ⋖ Φ ⇂ wf_fill P Φ) ⊨ btot (P ⋖ Ψ ⇂ wf_fill P Ψ).
+Lemma pgrounding : ∀ (P : pctx) (Φ Ψ : bouquet),
+  Φ ⊨ Ψ -> P ⋖ Φ ⊨ P ⋖ Ψ.
 Admitted.
 
-Lemma in_bouquet : ∀ (Φ : bouquet) (H H' : wf Φ) ϕ,
-  ϕ ∈ btot (Φ ⇂ H) <-> ϕ ∈ btot (Φ ⇂ H').
-Proof.
-  done.
-Qed.
-
-Lemma entails_refl (Φ : bouquet) (H H' : wf Φ) :
-  btot (Φ ⇂ H) ⊨ btot (Φ ⇂ H').
-Proof.
-  intros ?? Hf ϕ. by apply (Hf ϕ).
-Qed.
-
-Lemma eqentails_refl (Φ : bouquet) (H H' : wf Φ) :
-  btot (Φ ⇂ H) ⫤⊨ btot (Φ ⇂ H').
-Proof.
-  split; by apply entails_refl.
-Qed.
-
-Lemma wf_cstep {Φ Ψ : bouquet} :
-  Φ ≈> Ψ -> wf Φ -> wf Ψ.
-Admitted.
-
-Theorem soundness : ∀ (Φ Ψ : wfbouquet),
+Theorem soundness : ∀ (Φ Ψ : bouquet),
   Φ ≈>* Ψ -> Φ ⫤⊨ Ψ.
 Proof.
-  move => [Φ HΦ] [Ψ HΨ]. do 2 rewrite [bfgt _]/=.
-  induction 1 as [Φ |Φ1 Φ2 Φ3 Hstep H IH].
-  * by apply eqentails_refl.
-  * rewrite -(IH (wf_cstep Hstep HΦ) HΨ). admit.
 Admitted.
 
 End Soundness.
@@ -60,20 +32,20 @@ End Soundness.
 
 Section Completeness.
 
-Definition tderiv (T : theory) (ϕ : wfflower) :=
-  ∃ (Φ : wfbouquet), btot Φ ⊆ T /\ let 'Φ ⇂ _ := Φ in Φ ⊢ ϕ.
+Definition tderiv (T : theory) (ϕ : flower) :=
+  ∃ (Φ : bouquet), btot Φ ⊆ T /\ Φ ⊢ ϕ.
 
-Definition tnderiv (T : theory) (ϕ : wfflower) :=
-  ∀ (Φ : wfbouquet), btot Φ ⊆ T -> let 'Φ ⇂ _ := Φ in ~ (Φ ⊢ ϕ).
+Definition tnderiv (T : theory) (ϕ : flower) :=
+  ∀ (Φ : bouquet), btot Φ ⊆ T -> ~ (Φ ⊢ ϕ).
 
 Infix "!⊢" := tderiv (at level 70).
 Infix "!⊬" := tnderiv (at level 70).
 
-Definition consistent (ϕ : wfflower) (T : theory) :=
+Definition consistent (ϕ : flower) (T : theory) :=
   T !⊬ ϕ.
 
-Definition complete (ϕ : wfflower) (T : theory) :=
-  ∀ (ψ : wfflower), T ∪ ψ !⊢ ϕ \/ ψ ∈ T.
+Definition complete (ϕ : flower) (T : theory) :=
+  ∀ (ψ : flower), T ∪ ψ !⊢ ϕ \/ ψ ∈ T.
 
 Lemma completeness_contra T ϕ :
   T !⊬ ϕ -> ∃ A (K : KModel A), ~ (T ⊨ ϕ).
@@ -85,11 +57,11 @@ Proof.
   tauto.
 Qed.
 
-Lemma not_prov_tnderiv (ϕ : wfflower) :
+Lemma not_prov_tnderiv (ϕ : flower) :
   ~ prov ϕ -> ∅ !⊬ ϕ.
 Admitted.
 
-Theorem completeness (ϕ : wfflower) :
+Theorem completeness (ϕ : flower) :
   (∀ A (K : KModel A), ∅ ⊨ ϕ) -> prov ϕ.
 Proof.
   apply contra_recip. move => H H'. apply not_prov_tnderiv in H.
@@ -99,7 +71,7 @@ Qed.
 
 End Completeness.
 
-Theorem structural_admissibility (ϕ : wfflower) :
+Theorem structural_admissibility (ϕ : flower) :
   sprov ϕ -> prov ϕ.
 Proof.
   intros. apply completeness. intros.
