KripkeSemantics.v
@@ -2,213 +2,36 @@ Require Import ssreflect stdpp.boolset stdpp.propset stdpp.vector.
 
 Require Import Flowers.Utils Flowers.Terms Flowers.Syntax.
 
-(** * Well-formed terms with respect to a signature *)
+(** ** Theories are sets of flowers *)
 
-Record sig : Type := {
-  funs : boolset name;
-  preds : boolset name;
-  farity : ∀ f, f ∈ funs -> nat;
-  parity : ∀ p, p ∈ preds -> nat;
-}.
+Definition theory := propset flower.
 
-Context (Σ : sig).
+Definition btot (Φ : bouquet) : theory :=
+  {[ ϕ | ϕ ∈ Φ ]}.
 
-(* Fixpoint twf (t : term) : bool :=
-  match t with
-  | TVar _ => true
-  | TFun f args =>
-      match decide (f ∈ Σ.(funs)) with
-      | left w => (length args =? Σ.(farity) f w) && forallb (twf <$> args)
-      | right _ => false
-      end
-  end. *)
+#[global] Coercion btot : bouquet >-> theory.
 
-Inductive twf : term -> Type :=
-| twf_var n :
-    twf (TVar n)
-| twf_fun f args :
-    ∀ (Hf : f ∈ Σ.(funs)), ltwf args -> length args = Σ.(farity) f Hf ->
-    twf (TFun f args)
-with ltwf : list term -> Type :=
-| ltwf_nil :
-    ltwf []
-| ltwf_cons t l :
-    twf t -> ltwf l ->
-    ltwf (t :: l).
-
-Definition wfterm :=
-  { t : term & twf t }.
-
-(* Fixpoint wf (ϕ : flower) :=
-  match ϕ with
-  | Atom p args =>
-      match decide (p ∈ Σ.(preds)) with
-      | left w => (length args =? Σ.(parity) p w) && forallb (twf <$> args)
-      | right _ => false
-      end
-  | γ ⫐ Δ =>
-      let gwf '(n ⋅ Φ) := forallb (wf <$> Φ) in
-      gwf γ && forallb (gwf <$> Δ)
-  end. *)
-
-Inductive fwf : flower -> Type :=
-| fwf_atom p args :
-    ∀ (Hp : p ∈ Σ.(preds)), ltwf args -> length args = Σ.(parity) p Hp ->
-    fwf (Atom p args)
-| fwf_flower n Φ Δ :
-    wf Φ -> pwf Δ ->
-    fwf (n ⋅ Φ ⫐ Δ)
-with wf : bouquet -> Type :=
-| wf_nil : wf []
-| wf_cons ϕ Φ : fwf ϕ -> wf Φ -> wf (ϕ :: Φ)
-with pwf : list garden -> Type :=
-| pwf_nil : pwf []
-| pwf_cons n Φ Δ : wf Φ -> pwf Δ -> pwf ((n ⋅ Φ) :: Δ).
-
-Definition wfflower :=
-  { ϕ : flower & fwf ϕ }.
-
-Definition wfbouquet :=
-  { Φ : bouquet & wf Φ }.
-
-Definition wfctx :=
-  { X : ctx & wf X }.
-
-Definition wfpctx :=
-  { P : pctx & wf P }. 
-
-Definition ffgt : wfflower -> flower := projT1.
-Definition bfgt : wfbouquet -> bouquet := projT1.
-Definition cfgt : wfctx -> ctx := projT1.
-Definition pfgt : wfpctx -> pctx := projT1.
-Coercion ffgt : wfflower >-> flower.
-Coercion bfgt : wfbouquet >-> bouquet.
-Coercion cfgt : wfctx >-> ctx.
-(* Coercion pfgt : wfpctx >-> pctx. *)
-
-Definition wfpctx_to_wfctx : wfpctx -> wfctx := λ '(P ⇂ H), (pctx_to_ctx P) ⇂ H.
-Coercion wfpctx_to_wfctx : wfpctx >-> wfctx.
-
-Lemma wf_app (Φ Ψ : bouquet) :
-  wf Φ -> wf Ψ -> wf (Φ ++ Ψ).
-Proof.
-  elim => {Φ} [|ϕ Φ Hϕ HΦ IH] H //=.
-  econs.
-Qed.
-
-Lemma pwf_app (Γ Δ : list garden) :
-  pwf Γ -> pwf Δ -> pwf (Γ ++ Δ).
-Proof.
-  elim => {Γ} [|γ Γ Hγ HΓ IH] H //=.
-  econs.
-Qed.
-
-Lemma wf_app_inv : ∀ (Φ Ψ : bouquet),
-  wf (Φ ++ Ψ) -> wf Φ * wf Ψ.
-Proof.
-  elim => [|ϕ Φ IH] /= Ψ H; split.
-  econs. done.
-  econs. inv H.
-  inv H. by apply (IH Ψ).
-  inv H. by apply (IH Ψ).
-Qed.
-
-Lemma pwf_app_inv : ∀ (Γ Δ : list garden),
-  pwf (Γ ++ Δ) -> pwf Γ * pwf Δ.
-Proof.
-  elim => [|γ Γ IH] /= Δ H; split.
-  econs. done. destruct γ as [n Φ].
-  econs. inv H.
-  inv H. by apply (IH Δ).
-  inv H. by apply (IH Δ).
-Qed.
-
-Lemma wf_Planter_inv {X : ctx} {Φl Φr} :
-  wf (Planter Φl X Φr) -> wf Φl * wf X * wf Φr.
-Proof.
-  cbn. move => H.
-  case (wf_app_inv _ _ H) => {H} [Hl H];
-  case (wf_app_inv _ _ H) => {H} [HX Hr].
-  done.
-Qed.
-
-Lemma wf_Pistil_inv {X : ctx} {n Δ} :
-  wf (Pistil n X Δ) -> wf X * pwf Δ.
-Proof.
-  cbn. move => H. inv H. inv X0. done.
-Qed.
-
-Lemma wf_Petal_inv {X : ctx} {n Φ Δ m Δ'} :
-  wf (Petal (n ⋅ Φ) Δ m X Δ') -> wf Φ * pwf Δ * wf X * pwf Δ'.
-Proof.
-  cbn. move => H. inv H. inv X0.
-  case (pwf_app_inv _ _ X3) => HΔ H. rewrite cons_app in H.
-  case (pwf_app_inv _ _ H) => HX HΔ'. inv HX.
-  done.
-Qed.
-
-Lemma wf_fill : ∀ (X : wfctx) (Φ : wfbouquet),
-  wf (X ⋖ Φ).
-Proof.
-  move => []/=.
-  elim => [|Φl X IH Φr |n X IH Δ |γ Δ n X IH Δ'] H [Φ HΦ] //=.
-
-  case (wf_Planter_inv H); move => [Hl HX] Hr.
-  repeat apply wf_app. done. by apply (IH HX (Φ ⇂ HΦ)). done.
-
-  case (wf_Pistil_inv H); move => HX HΔ.
-  econs; econs. apply (IH HX (Φ ⇂ HΦ)).
-
-  destruct γ as [m Ψ].
-  case (wf_Petal_inv H); move => [[HΨ HΔ] HX] HΔ'.
-  econs; econs. rewrite cons_app. repeat apply pwf_app.
-  done. econs. apply (IH HX (Φ ⇂ HΦ)). econs. done.
-Qed.
-
-(** ** Theories are sets of well-formed flowers *)
-
-Definition theory := propset wfflower.
-
-Definition ftot (ϕ : wfflower) : theory :=
-  {[ ϕ ]}.
-
-Definition btot (Φ : wfbouquet) : theory :=
-  {[ ϕ | ffgt ϕ ∈ bfgt Φ ]}.
-
-#[global] Coercion ftot : wfflower >-> theory.
-#[global] Coercion btot : wfbouquet >-> theory.
-
-(** * Pre-models are just domains with interpretation functions for well-formed
-      terms *)
+(** * Pre-models are just domains with interpretation functions for terms and
+      predicates *)
 
 Definition elem {A C} `{Set_ A C} (X : C) :=
   { x | x ∈ X }.
 
 Class premodel (D : Type) := {
   domain : propset D;
-  interp_fun : ∀ (f : name) (H : f ∈ Σ.(funs)),
-    vec (elem domain) (Σ.(farity) f H) -> elem domain;
-  interp_pred : ∀ (p : name) (H : p ∈ Σ.(preds)),
-    propset (vec (elem domain) (Σ.(parity) p H));
+  interp_fun : name -> list (elem domain) -> elem domain;
+  interp_pred : name -> propset (list (elem domain))
 }.
 
-Definition elem_subseteq {A : Type} (X Y : propset A) :
+Definition elem_subseteq {A : Type} {X Y : propset A} :
   X ⊆ Y -> elem X -> elem Y.
 Proof.
   move => H [x Hx]. exists x. exact (H x Hx).
 Defined.
 
-Definition elem_subseteq_vec {A : Type} (X Y : propset A) :
-  X ⊆ Y -> ∀ n, vec (elem X) n -> vec (elem Y) n.
-Proof.
-  move => H. elim => [|n IH] xs.
-  * exact [#].
-  * inversion xs using (@vec_S_inv (elem X)).
-    move => {xs} [x Hx] xs.
-    constructor.
-    - exists x. exact (H x Hx).
-    - exact (IH xs).
-Defined.
+Definition elem_subseteq_list {A : Type} {X Y : propset A}
+    (H : X ⊆ Y) (l : list (elem X)) : list (elem Y) :=
+  (λ '(x ↾ Hx), x ↾ H x Hx) <$> l.
 
 (* Pre-model inclusion is domain and interpretation inclusion *)
 
@@ -216,12 +39,12 @@ Definition premodel_incl {D} (M1 M2 : premodel D) : Prop.
 Proof.
   refine { H : M1.(domain) ⊆ M2.(domain) | _ }.
   refine (_ /\ _).
-  * refine (∀ (f : name) (Hf : f ∈ Σ.(funs)) (args : vec (elem M1.(domain)) (Σ.(farity) f Hf)), _ =@{elem M2.(domain)} _).
-    refine (elem_subseteq _ _ H (M1.(interp_fun) f Hf args)).
-    refine (M2.(interp_fun) f Hf (elem_subseteq_vec _ _ H _ args)).
-  * refine (∀ (p : name) (Hp : p ∈ Σ.(preds)) (args : vec (elem M1.(domain)) (Σ.(parity) p Hp)), impl _ _).
-    refine (args ∈ M1.(interp_pred) p Hp).
-    refine ((elem_subseteq_vec _ _ H _ args) ∈ M2.(interp_pred) p Hp).
+  * refine (∀ (f : name) (args : list (elem M1.(domain))), _ =@{elem M2.(domain)} _).
+    refine (elem_subseteq H (M1.(interp_fun) f args)).
+    refine (M2.(interp_fun) f (elem_subseteq_list H args)).
+  * refine (∀ (p : name) (args : list (elem M1.(domain))), impl _ _).
+    refine (args ∈ M1.(interp_pred) p).
+    refine ((elem_subseteq_list H args) ∈ M2.(interp_pred) p).
 Defined.
 
 (** * Term evaluation in a given pre-model *) 
@@ -237,17 +60,11 @@ Definition eval := nat -> dom.
 Definition update (n : nat) (e1 e2 : eval) :=
   fun m => if m <? n then e1 m else e2 (m - n).
 
-Fixpoint lapply_eval (e : eval) (l : list term) (H : ltwf l) {struct H} : vec dom (length l) :=
-  match H with
-  | ltwf_nil => vnil
-  | ltwf_cons x l Hx Hl =>
-      vcons (tapply_eval e x Hx) (lapply_eval e l Hl)
-  end
-with tapply_eval (e : eval) (t : term) (H : twf t) {struct H} : dom :=
-  match H with
-  | twf_var n => e n
-  | twf_fun f args Hf Hargs Hlen =>
-      interp_fun f Hf (vec_resize Hlen (lapply_eval e args Hargs))
+Fixpoint tapply_eval (e : eval) (t : term) {struct t} : dom :=
+  match t with
+  | TVar n => e n
+  | TFun f args =>
+      interp_fun f (tapply_eval e <$> args)
   end.
 
 End Eval.
@@ -275,77 +92,41 @@ Section Forcing.
 
 Context {D} {K : KModel D}.
 
-Lemma eval_incl {α β} :
-  α ≤ β -> eval (model α) -> eval (model β).
+Lemma eval_incl {w w'} :
+  w ≤ w' -> eval (model w) -> eval (model w').
 Proof.
   move => H e.
   refine (fun n => _).
-  case (model_mono α β H) => [Hincl _].
+  case (model_mono w w' H) => [Hincl _].
   case (e n) => [a Ha].
   exists a. by apply Hincl.
 Defined.
 
-(* Reserved Notation "α : e ⊩f ϕ" (at level 20, e at level 0).
-Reserved Notation "α : e ⊩ Φ" (at level 20, e at level 0).
-Reserved Notation "α : e ⊩p Δ" (at level 20, e at level 0).
-
-Inductive forces (α : world) (e : eval (model α)) : flower -> Prop :=
-
-| forces_atom p args Hp Hargs Hlen :
-    (vec_resize Hlen (lapply_eval (model α) e args Hargs)) ∈ interp_pred p Hp ->
-    α : e ⊩f Atom p args
-
-| forces_flower n Φ Δ :
-    (∀ β (H : α ≤ β), ∀ (en : eval (model β)),
-     let e' := update (model β) n en (eval_incl H e) in
-     β : e' ⊩ Φ -> β : e' ⊩p Δ) ->
-    α : e ⊩f (n ⋅ Φ ⫐ Δ)
-
-with bforces (α : world) (e : eval (model α)) : bouquet -> Prop :=
-
-with pforces (α : world) (e : eval (model α)) : list garden -> Prop :=
-
-where "α : e ⊩f ϕ" := (forces α e ϕ)
-  and "α : e ⊩ Φ" := (bforces α e Φ)
-  and "α : e ⊩p Δ" := (pforces α e Δ). *)
-
-Reserved Notation "α : e ⊩f ϕ ! H" (at level 20, e at level 0).
-Reserved Notation "α : e ⊩b Φ ! H" (at level 20, e at level 0).
-Reserved Notation "α : e ⊩p Δ ! H" (at level 20, e at level 0).
-
-Fixpoint fforces (α : world) (e : eval (model α)) (ϕ : flower) (H : fwf ϕ) : Prop :=
-  match H with
-  | fwf_atom p args Hp Hargs Hlen =>
-      (vec_resize Hlen (lapply_eval (model α) e args Hargs)) ∈ interp_pred p Hp
-  | fwf_flower n Φ Δ HΦ HΔ =>
-      ∀ β (H : α ≤ β), ∀ (en : eval (model β)),
-      let e' := update (model β) n en (eval_incl H e) in
-      β : e' ⊩b Φ ! HΦ -> β : e' ⊩p Δ ! HΔ
-  end
-
-with bforces (α : world) (e : eval (model α)) (Φ : bouquet) (H : wf Φ) : Prop :=
-  match H with
-  | wf_nil =>
-      True
-  | wf_cons ϕ Φ Hϕ HΦ =>
-      α : e ⊩f ϕ ! Hϕ /\ α : e ⊩b Φ ! HΦ
-  end
-
-with pforces (α : world) (e : eval (model α)) (Δ : list garden) (H : pwf Δ) : Prop :=
-  match H with
-  | pwf_nil =>
-      False
-  | pwf_cons n Φ Δ HΦ HΔ =>
-      (∃ (en : eval (model α)), α : (update (model α) n en e) ⊩b Φ ! HΦ) \/
-      α : e ⊩p Δ ! HΔ
-  end
-
-where "α : e ⊩f ϕ ! H" := (fforces α e ϕ H)
-  and "α : e ⊩b Φ ! H" := (bforces α e Φ H)
-  and "α : e ⊩p Δ ! H" := (pforces α e Δ H).
+Fixpoint fforces (w : world) (e : eval (model w)) (ϕ : flower) {struct ϕ} : Prop :=
+  let fix bforces w e Φ :=
+    match Φ with
+    | [] => True
+    | ϕ :: Φ =>
+        fforces w e ϕ /\ bforces w e Φ
+    end in
+  let fix pforces w e Δ :=
+    match Δ with
+    | [] => False
+    | (n ⋅ Φ) :: Δ =>
+        (∃ (en : eval (model w)), bforces w (update (model w) n en e) Φ) \/
+        pforces w e Δ
+    end in
+  match ϕ with
+  | Atom p args =>
+      tapply_eval (model w) e <$> args ∈ interp_pred p
+  | Flower (n ⋅ Φ) Δ =>
+      ∀ w' (H : w ≤ w'), ∀ (en : eval (model w')),
+      let e' := update (model w') n en (eval_incl H e) in
+      bforces w' e' Φ -> pforces w' e' Δ
+  end.
 
 Definition forces α e (T : theory) :=
-  ∀ ϕ, ϕ ∈ T -> let 'ϕ ⇂ H := ϕ in α : e ⊩f ϕ ! H.
+  ∀ ϕ, ϕ ∈ T -> fforces α e ϕ.
 
 Notation "α : e ⊩ T" := (forces α e T) (at level 20, e at level 0).
 
@@ -364,7 +145,7 @@ Proof.
     apply HBA. by apply HCB.
 Qed.
 
-#[export] Instance : Equiv wfbouquet := eqentails.
+#[export] Instance : Equiv bouquet := eqentails.
 
 End Forcing.
 
